Experiment failed

mechanization/theories/PtsSignature.v
@@ -1,7 +1,14 @@
 From Coq Require Import Relation_Definitions RelationClasses.
-From McPTS.Core.PTSSignature Require Import Signature.
 
+(* Pure type system signatures consist of sorts, axioms, and rules *)
+Record PtsSig : Type :=
+  mkPtsSig{
+      St : Set;
+      Ax : St -> St -> Set;
+      Ru : St -> St -> St -> Set;
+    }.
 
+(* A signature is predicative if there is a partial order that respects its relations *)
 Record PredicativeSig (S : PtsSig) : Prop :=
   mkPredicativeSig {
       test : exists (P : relation (St S)),
