mechanization/theories/Core/Syntactic/System/Definitions.v
@@ -1,72 +1,72 @@
 From Coq Require Import List Classes.RelationClasses Setoid Morphisms.
 
+From McPTS Require Import PtsSignature.
 From McPTS.Core Require Import Base.
-From McPTS.Core.PTSSignature Require Import Signature.
 From McPTS.Core.Syntactic Require Export Syntax.
 
 Reserved Notation "⊢ Γ" (in custom judg at level 80, Γ custom Exp).
 Reserved Notation "⊢ Γ ≡ Δ" (in custom judg at level 80, Γ custom Exp, Δ custom Exp).
-Reserved Notation "Γ ⊢ M : A" (in custom judg at level 80, Γ custom Exp, M custom Exp, A custom Exp).
-Reserved Notation "Γ ⊢ M ≡ N : A" (in custom judg at level 80, Γ custom Exp, M custom Exp, N custom Exp, A custom Exp).
-Reserved Notation "Γ ⊢ A" (in custom judg at level 80, Γ custom Exp, A custom Exp).
-Reserved Notation "Γ ⊢ A ≡ B" (in custom judg at level 80, Γ custom Exp, A custom Exp, B custom Exp).
+Reserved Notation "Γ ⊢ M : A :: K" (in custom judg at level 80, Γ custom Exp, M custom Exp, A custom Exp, K custom Exp).
+Reserved Notation "Γ ⊢ M ≡ N : A :: K" (in custom judg at level 80, Γ custom Exp, M custom Exp, N custom Exp, A custom Exp, K custom Exp).
+Reserved Notation "Γ ⊢ A :: K" (in custom judg at level 80, Γ custom Exp, A custom Exp, K custom Exp).
+Reserved Notation "Γ ⊢ A ≡ B :: K" (in custom judg at level 80, Γ custom Exp, A custom Exp, B custom Exp, K custom Exp).
 Reserved Notation "Γ ⊢s σ : Δ" (in custom judg at level 80, Γ custom Exp, σ custom Exp, Δ custom Exp).
 Reserved Notation "Γ ⊢s σ ≡ τ : Δ" (in custom judg at level 80, Γ custom Exp, σ custom Exp, τ custom Exp, Δ custom Exp).
-Reserved Notation "'#' x : A : s ∈ Γ" (in custom judg at level 80, x constr at level 0, A custom Exp, s custom Exp, Γ custom Exp).
+Reserved Notation "'#' x : A :: K ∈ Γ" (in custom judg at level 80, x constr at level 0, A custom Exp, K custom Exp, Γ custom Exp).
 
 Generalizable All Variables.
 
-(* Context lookup: #x : A : S ∈ Γ *)
-Inductive ctx_lookup {P : PtsSig} : nat -> Typ P -> St P -> Ctx P -> Prop :=
-| here : `({{ #0 : [Wk]A : s ∈ Γ, A : s }})
-| there : `({{ #i : A : s ∈ Γ }} ->
-            {{ #(S i) : [Wk]A : s ∈ Γ, B : s}})
-where "'#' x : A : s ∈ Γ" := (ctx_lookup x A s Γ) (in custom judg) : type_scope.
+(* Context lookup: #x : A :: Sort@s ∈ Γ *)
+Inductive ctx_lookup {P : PtsSig} : nat -> Typ P -> Knd P -> Ctx P -> Prop :=
+| here : `({{ #0 : [Wk]A :: Sort@s ∈ Γ, A :: Sort@s }})
+| there : `({{ #i : A :: Sort@s ∈ Γ }} ->
+            {{ #(S i) : [Wk]A :: Sort@s ∈ Γ, B :: Sort@s'}})
+where "'#' x : A :: K ∈ Γ" := (ctx_lookup x A K Γ) (in custom judg) : type_scope.
 
 (* Context formation: ⊢ Γ *)
 Inductive wf_ctx {P : PtsSig} : Ctx P -> Prop :=
 | wf_ctx_empty : {{ ⊢ ⋅ }}
-| wf_ctx_extend : `({{ ⊢ Γ }} -> {{ Γ ⊢ A : Sort@s}} ->
-                    {{ ⊢ Γ, A:s}})
+| wf_ctx_extend : `({{ ⊢ Γ }} -> {{ Γ ⊢ A :: Sort@s }} ->
+                    {{ ⊢ Γ, A :: Sort@s}})
 where "⊢ Γ" := (wf_ctx Γ) (in custom judg) : type_scope
 
 (* Typing for expressions: Γ ⊢ M : A *)
-with wf_exp {P : PtsSig} : Ctx P -> Exp P -> Typ P -> Prop :=
+with wf_exp {P : PtsSig} : Ctx P -> Exp P -> Typ P -> Knd P -> Prop :=
 | wf_exp_st : `(Ax P s1 s2 -> {{ ⊢ Γ }} -> 
-                {{ Γ ⊢ Sort@s1 : Sort@s2 }})
-| wf_exp_var : `({{ ⊢ Γ }} -> {{ #i : A : s ∈ Γ }} ->
-                 {{ Γ ⊢ #i : A}})
+                {{ Γ ⊢ Sort@s1 : Sort@s2 :: Type}})
+| wf_exp_var : `({{ ⊢ Γ }} -> {{ #i : A :: Sort@s ∈ Γ }} ->
+                 {{ Γ ⊢ #i : A :: Sort@s}})
 | wf_exp_pi : `(forall r : Ru P s1 s2 s3,
-                    {{ Γ ⊢ A : Sort@s1 }} -> {{ Γ, A:s1 ⊢ B : Sort@s2 }} ->
-                    {{ Γ ⊢ Π r A B : Sort@s3 }})
+                    {{ Γ ⊢ A : Sort@s1 :: Type }} -> {{ Γ, A :: Sort@s1 ⊢ B : Sort@s2 :: Type }} ->
+                    {{ Γ ⊢ Π r A B : Sort@s3 :: Type}})
 | wf_exp_lam : `(forall r : Ru P s1 s2 s3,
-                     {{ Γ ⊢ Π r A B : Sort@s3 }} -> {{ Γ, A:s ⊢ M : B }} ->
-                     {{ Γ ⊢ λM : Π r A B }})
+                     {{ Γ ⊢ Π r A B : Sort@s3 :: Type}} -> {{ Γ, A :: Sort@s ⊢ M : B :: Sort@s2 }} ->
+                     {{ Γ ⊢ λM : Π r A B :: Sort@s3}})
 | wf_exp_app : `(forall r : Ru P s1 s2 s3,
-                     {{ Γ ⊢ Π r A B : Sort@s3 }} -> {{ Γ ⊢ M : Π r A B }} -> {{ Γ ⊢ N : A }} ->
-                     {{ Γ ⊢ M N : [Id,,N]B }})
-| wf_exp_clo : `({{ Γ ⊢s σ : Δ }} -> {{ Δ ⊢ M : A }} ->
-                 {{ Γ ⊢ [σ]M : [σ]A }})
-| wf_exp_conv : `({{ Γ ⊢ M : A }} -> {{ Γ ⊢ A ≡ B }} ->
-                  {{ Γ ⊢ M : B }})
-where "Γ ⊢ M : A" := (wf_exp Γ M A) (in custom judg) : type_scope
+                     {{ Γ ⊢ Π r A B : Sort@s3 :: Type }} -> {{ Γ ⊢ M : Π r A B :: Sort@s3 }} -> {{ Γ ⊢ N : A :: Sort@s1 }} ->
+                     {{ Γ ⊢ M N : [Id,,N]B :: Sort@s2 }})
+| wf_exp_clo : `({{ Γ ⊢s σ : Δ }} -> {{ Δ ⊢ M : A :: K }} ->
+                 {{ Γ ⊢ [σ]M : [σ]A :: K }})
+| wf_exp_conv : `({{ Γ ⊢ M : A :: K }} -> {{ Γ ⊢ A ≡ B : K :: L }} ->
+                  {{ Γ ⊢ M : B :: K }})
+where "Γ ⊢ M : A :: K" := (wf_exp Γ M A K) (in custom judg) : type_scope
 
-(* Type well-formedness: Γ ⊢ A *)
-with wf_typ {P : PtsSig} : Ctx P -> Typ P -> Prop :=
+(* Type well-formedness: Γ ⊢ A :: K *)
+with wf_typ {P : PtsSig} : Ctx P -> Typ P -> Knd P -> Prop :=
 | wf_typ_st : `({{ ⊢ Γ }} ->
-                {{ Γ ⊢ Sort@s }})
-| wf_typ_exp : `({{ Γ ⊢ A : Sort@s }} ->
-                 {{ Γ ⊢ A }})
-where "Γ ⊢ A" := (wf_typ Γ A) (in custom judg) : type_scope
+                {{ Γ ⊢ Sort@s :: Type }})
+| wf_typ_exp : `({{ Γ ⊢ A : Sort@s :: K }} ->
+                 {{ Γ ⊢ A :: Sort@s }})
+where "Γ ⊢ A :: K" := (wf_typ Γ A K) (in custom judg) : type_scope
 
 (* Typing for substitutions: Γ ⊢s σ : Δ *)
 with wf_sub {P : PtsSig} : Ctx P -> Sub P -> Ctx P -> Prop :=
 | wf_sub_id : `({{ ⊢ Γ }} ->
                 {{ Γ ⊢s Id : Γ }})
-| wf_sub_wk : `({{ ⊢ Γ, A:s }} ->
-                {{ Γ, A:s ⊢s Wk : Γ }})
-| wf_sub_ext : `({{ Γ ⊢s σ : Δ }} -> {{ Δ ⊢ A : Sort@s }} -> {{ Γ ⊢ M : [σ]A }} ->
-                 {{ Γ ⊢s σ,,M : Δ, A:s }})
+| wf_sub_wk : `({{ ⊢ Γ, A :: Sort@s }} ->
+                {{ Γ, A :: Sort@s ⊢s Wk : Γ }})
+| wf_sub_ext : `({{ Γ ⊢s σ : Δ }} -> {{ Δ ⊢ A : Sort@s :: Type }} -> {{ Γ ⊢ M : [σ]A :: Sort@s }} ->
+                 {{ Γ ⊢s σ,,M : Δ, A :: Sort@s }})
 | wf_sub_comp : `({{ Γ1 ⊢s σ : Γ2 }} -> {{ Γ2 ⊢s τ :Γ3 }} ->
                   {{ Γ1 ⊢s σ ∘ τ : Γ3 }})
 | wf_sub_conv : `({{ Γ ⊢s σ : Δ }} -> {{ ⊢ Δ ≡ Δ' }} ->
@@ -77,81 +77,82 @@ where "Γ ⊢s σ : Δ" := (wf_sub Γ σ Δ) (in custom judg) : type_scope
 with eq_ctx {P : PtsSig} : Ctx P -> Ctx P -> Prop :=
 | eq_ctx_nil : {{ ⊢ ⋅ ≡ ⋅ }}
 | eq_ctx_cons : `({{ ⊢ Γ ≡ Δ }} ->
-                  {{ Γ ⊢ A : Sort@s }} -> {{ Γ ⊢ B : Sort@s }} ->
-                  {{ Δ ⊢ A : Sort@s }} -> {{ Δ ⊢ B : Sort@s }} ->
-                  {{ Γ ⊢ A ≡ B : Sort@s }} ->
-                  {{ ⊢ Γ, A:s ≡ Δ, B:s }})
+                  {{ Γ ⊢ A :: Sort@s }} -> {{ Γ ⊢ B :: Sort@s }} ->
+                  {{ Δ ⊢ A :: Sort@s }} -> {{ Δ ⊢ B :: Sort@s }} ->
+                  {{ Γ ⊢ A ≡ B :: Sort@s }} ->
+                  {{ Δ ⊢ A ≡ B :: Sort@s }} ->
+                  {{ ⊢ Γ, A :: Sort@s ≡ Δ, B :: Sort@s }})
 where "⊢ Γ ≡ Δ" := (eq_ctx Γ Δ) (in custom judg) : type_scope
 
 (* Expressions equality: Γ ⊢ M ≡ N : A *)
-with eq_exp {P : PtsSig} : Ctx P -> Exp P -> Exp P -> Typ P -> Prop :=
+with eq_exp {P : PtsSig} : Ctx P -> Exp P -> Exp P -> Typ P -> Knd P -> Prop :=
 (* β-reduction and η-expansion *)
 | eq_exp_beta : `(forall r : Ru P s1 s2 s3,
-                      {{ Γ ⊢ Π r A B : Sort@s3 }} -> {{ Γ, A:s1 ⊢ M : B }} -> {{ Γ ⊢ N : A }} ->
-                      {{ Γ ⊢ M N ≡ [Id,,N]M : [Id,,N]B }})
+                      {{ Γ ⊢ Π r A B : Sort@s3 :: K }} -> {{ Γ, A :: Sort@s1 ⊢ M : B :: Sort@s2 }} -> {{ Γ ⊢ N : A :: Sort@s1 }} ->
+                      {{ Γ ⊢ M N ≡ [Id,,N]M : [Id,,N]B :: Sort@s2 }})
 | eq_exp_eta : `(forall r : Ru P s1 s2 s3,
-                     {{ Γ ⊢ Π r A B : Sort@s3 }} -> {{ Γ ⊢ M : Π r A B }} ->
-                     {{ Γ ⊢ M ≡ λ([Wk]M #0) : Π r A B }})
+                     {{ Γ ⊢ Π r A B : Sort@s3 :: K }} -> {{ Γ ⊢ M : Π r A B :: Sort@s3 }} ->
+                     {{ Γ ⊢ M ≡ λ([Wk]M #0) : Π r A B :: Sort@s3 }})
 (* Substitution propagation *)
 | eq_exp_prop_sort : `(Ax P s1 s2 -> {{ Γ ⊢s σ : Δ }} ->
-                       {{ Γ ⊢ [σ]Sort@s1 ≡ Sort@s1 : Sort@s2 }})
-| eq_exp_prop_var_ze : `({{ Γ ⊢s σ,,M : Δ, A:s }} ->
-                         {{ Γ ⊢ [σ,,M]#0 ≡ M : [σ]A }})
-| eq_exp_prop_var_su : `({{ Γ ⊢s σ,,M : Δ, A:s1 }} -> {{ #i:B:s2 ∈ Δ }} ->
-                         {{ Γ ⊢ [σ,,M]#(S i) ≡ [σ]#i : [σ]B }})
+                       {{ Γ ⊢ [σ]Sort@s1 ≡ Sort@s1 : Sort@s2 :: Type }})
+| eq_exp_prop_var_ze : `({{ Γ ⊢s σ,,M : Δ, A :: Sort@s }} ->
+                         {{ Γ ⊢ [σ,,M]#0 ≡ M : [σ]A :: Sort@s }})
+| eq_exp_prop_var_su : `({{ Γ ⊢s σ,,M : Δ, A :: Sort@s1 }} -> {{ #i : B :: Sort@s2 ∈ Δ }} ->
+                         {{ Γ ⊢ [σ,,M]#(S i) ≡ [σ]#i : [σ]B :: Sort@s2 }})
 | eq_exp_prop_pi : `(forall r : Ru P s1 s2 s3,
-                         {{ Γ ⊢s σ : Δ }} -> {{ Δ ⊢ Π r A B : Sort@s3 }} ->
-                         {{ Γ ⊢ [σ](Π r A B) ≡ Π r ([σ] A) ([(Wk ∘ σ),,#0]B) : Sort@s3 }})
+                         {{ Γ ⊢s σ : Δ }} -> {{ Δ ⊢ Π r A B : Sort@s3 :: K }} ->
+                         {{ Γ ⊢ [σ](Π r A B) ≡ Π r ([σ] A) ([(Wk ∘ σ),,#0]B) : Sort@s3 :: K }})
 | eq_exp_prop_lam : `(forall r : Ru P s1 s2 s3,
-                          {{ Γ ⊢s σ : Δ }} -> {{ Δ ⊢ Π r A B : Sort@s3 }} -> {{ Δ, A:s1 ⊢ M : B }} ->
-                          {{ Γ ⊢ [σ](λM) ≡ λ([(Wk∘σ),,#0]M) : [σ](Π r A B) }})
+                          {{ Γ ⊢s σ : Δ }} -> {{ Δ ⊢ Π r A B : Sort@s3 :: K }} -> {{ Δ, A :: Sort@s1 ⊢ M : B :: Sort@s2 }} ->
+                          {{ Γ ⊢ [σ](λM) ≡ λ([(Wk∘σ),,#0]M) : [σ](Π r A B) :: Sort@s3 }})
 | eq_exp_prop_app : `(forall r : Ru P s1 s2 s3,
-                          {{ Γ ⊢s σ : Δ }} -> {{ Δ ⊢ Π r A B : Sort@s3 }} -> {{ Δ ⊢ M : Π r A B }} -> {{ Δ ⊢ N : A }} ->
-                          {{ Γ ⊢ [σ](M N) ≡ [σ]M [σ]N : [σ,,[σ]N]B }})
-| eq_exp_prop_id : `({{ Γ ⊢ M : A }} ->
-                     {{ Γ ⊢ [Id]M ≡ M : A }})
-| eq_exp_prop_comp : `({{ Γ1 ⊢s σ1 : Γ2 }} -> {{ Γ2 ⊢s σ2 : Γ3 }} -> {{ Γ3 ⊢ M : A }} ->
-                       {{ Γ1 ⊢ [σ1 ∘ σ2]M ≡ [σ1][σ2]M : [σ1 ∘ σ2]A }})
+                          {{ Γ ⊢s σ : Δ }} -> {{ Δ ⊢ Π r A B : Sort@s3 :: K }} -> {{ Δ ⊢ M : Π r A B:: Sort@s3 }} -> {{ Δ ⊢ N : A :: Sort@s1 }} ->
+                          {{ Γ ⊢ [σ](M N) ≡ [σ]M [σ]N : [σ,,[σ]N]B :: Sort@s2 }})
+| eq_exp_prop_id : `({{ Γ ⊢ M : A :: Sort@s }} ->
+                     {{ Γ ⊢ [Id]M ≡ M : A :: Sort@s }})
+| eq_exp_prop_comp : `({{ Γ1 ⊢s σ1 : Γ2 }} -> {{ Γ2 ⊢s σ2 : Γ3 }} -> {{ Γ3 ⊢ M : A :: Sort@s }} ->
+                       {{ Γ1 ⊢ [σ1 ∘ σ2]M ≡ [σ1][σ2]M : [σ1 ∘ σ2]A :: Sort@s }})
 (* Congruence rules *)
 | eq_exp_cong_pi : `(forall r : Ru P s1 s2 s3,
-                         {{ Γ ⊢ A1 ≡ A2 : Sort@s1 }} -> {{ Γ, A1:s1 ⊢ B1 ≡ B2 : Sort@s2 }} ->
-                         {{ Γ ⊢ Π r A1 B1 ≡ Π r A2 B2 : Sort@s3 }})
+                         {{ Γ ⊢ A1 ≡ A2 : Sort@s1 :: K }} -> {{ Γ, A1 :: Sort@s1 ⊢ B1 ≡ B2 : Sort@s2 :: K }} ->
+                         {{ Γ ⊢ Π r A1 B1 ≡ Π r A2 B2 : Sort@s3 :: K }})
 | eq_exp_cong_lam : `(forall r : Ru P s1 s2 s3,
-                          {{ Γ ⊢ Π r A B : Sort@s3 }} -> {{ Γ, A:s1 ⊢ M1 ≡ M2 : B }} ->
-                          {{ Γ ⊢ λM1 ≡ λM2 : Π r A B }})
+                          {{ Γ ⊢ Π r A B : Sort@s3 :: K }} -> {{ Γ, A :: Sort@s1 ⊢ M1 ≡ M2 : B :: Sort@s2 }} ->
+                          {{ Γ ⊢ λM1 ≡ λM2 : Π r A B :: Sort@s3 }})
 | eq_exp_cong_app : `(forall r : Ru P s1 s2 s3,
-                          {{ Γ ⊢ Π r A B : Sort@s3 }} -> {{ Γ ⊢ M1 ≡ M2 : Π r A B }} -> {{ Γ ⊢ N1 ≡ N2 : A }} ->
-                          {{ Γ ⊢ M1 N1 ≡ M2 N2 : [Id,,N1]B }})
-| eq_exp_cong_clo : `({{ Γ ⊢s σ1 ≡ σ2 : Δ }} -> {{ Δ ⊢ M1 ≡ M2 : A }} ->
-                      {{ Γ ⊢ [σ1]M1 ≡ [σ2]M2 : [σ1]A }})
+                          {{ Γ ⊢ Π r A B : Sort@s3 :: K }} -> {{ Γ ⊢ M1 ≡ M2 : Π r A B :: Sort@s3 }} -> {{ Γ ⊢ N1 ≡ N2 : A :: Sort@s1 }} ->
+                          {{ Γ ⊢ M1 N1 ≡ M2 N2 : [Id,,N1]B :: Sort@s2 }})
+| eq_exp_cong_clo : `({{ Γ ⊢s σ1 ≡ σ2 : Δ }} -> {{ Δ ⊢ M1 ≡ M2 : A :: Sort@s }} ->
+                      {{ Γ ⊢ [σ1]M1 ≡ [σ2]M2 : [σ1]A :: Sort@s }})
 (* Equivalence relation rules *)
-| eq_exp_refl : `({{ Γ ⊢ M : A }} ->
-                  {{ Γ ⊢ M ≡ M : A }})
-| eq_exp_sym : `({{ Γ ⊢ M1 ≡ M2 : A }} ->
-                 {{ Γ ⊢ M2 ≡ M1 : A }})
-| eq_exp_trans : `({{ Γ ⊢ M1 ≡ M2 : A }} -> {{ Γ ⊢ M2 ≡ M3 : A }} ->
-                   {{ Γ ⊢ M1 ≡ M3 : A }})
+| eq_exp_refl : `({{ Γ ⊢ M : A :: K }} ->
+                  {{ Γ ⊢ M ≡ M : A :: K }})
+| eq_exp_sym : `({{ Γ ⊢ M1 ≡ M2 : A :: K }} ->
+                 {{ Γ ⊢ M2 ≡ M1 : A :: K }})
+| eq_exp_trans : `({{ Γ ⊢ M1 ≡ M2 : A :: K }} -> {{ Γ ⊢ M2 ≡ M3 : A :: K }} ->
+                   {{ Γ ⊢ M1 ≡ M3 : A :: K }})
 (* Conversion rule *)
-| eq_exp_conv : `({{ Γ ⊢ M1 ≡ M2 : A }} -> {{ Γ ⊢ A ≡ B }} ->
-                  {{ Γ ⊢ M1 ≡ M2 : B }})
-where "Γ ⊢ M ≡ N : A" := (eq_exp Γ M N A) (in custom judg) : type_scope
+| eq_exp_conv : `({{ Γ ⊢ M1 ≡ M2 : A :: K }} -> {{ Γ ⊢ A ≡ B : K :: L }} ->
+                  {{ Γ ⊢ M1 ≡ M2 : B :: K }})
+where "Γ ⊢ M ≡ N : A :: K" := (eq_exp Γ M N A K) (in custom judg) : type_scope
 
 (* Type equality: Γ ⊢ A ≡ B *)
-with eq_typ {P : PtsSig} : Ctx P -> Typ P -> Typ P -> Prop :=
+with eq_typ {P : PtsSig} : Ctx P -> Typ P -> Typ P -> Knd P -> Prop :=
 | eq_typ_st : `({{ ⊢ Γ }} ->
-                {{ Γ ⊢ Sort@s ≡ Sort@s }})
-| eq_typ_exp : `({{ Γ ⊢ A ≡ B : Sort@s }} ->
-                 {{ Γ ⊢ A ≡ B }})
-where "Γ ⊢ A ≡ B" := (eq_typ Γ A B) (in custom judg) : type_scope
+                {{ Γ ⊢ Sort@s ≡ Sort@s :: Type }})
+| eq_typ_exp : `({{ Γ ⊢ A ≡ B : Sort@s :: K }} ->
+                 {{ Γ ⊢ A ≡ B :: Sort@s }})
+where "Γ ⊢ A ≡ B :: K" := (eq_typ Γ A B K) (in custom judg) : type_scope
 
 (* Substitution equality: Γ ⊢s σ ≡ τ : Δ *)
-with eq_sub {P : PtsSig} : Ctx P -> Sub P -> Sub P -> Ctx P -> Prop :=
+with eq_sub {P : PtsSig} : Ctx P -> Ctx P -> Sub P -> Sub P -> Prop :=
 (* β-reduction and η-expansion *)
 | eq_sub_beta_nil : `({{ ⋅ ⊢s Id ≡ .. : ⋅ }})
-| eq_sub_beta_cons : `({{ ⊢ Γ, A:s }} ->
-                       {{ Γ, A:s ⊢s Id ≡ (Wk ∘ Id),,#0 : Γ, A:s }})
-| eq_sub_eta : `({{ Γ ⊢s σ : Δ, A:s }} ->
-                 {{ Γ ⊢s σ ≡ (σ ∘ Wk),,[σ]#0 : Δ, A:s }})
+| eq_sub_beta_cons : `({{ ⊢ Γ, A :: Sort@s }} ->
+                       {{ Γ, A :: Sort@s ⊢s Id ≡ (Wk ∘ Id),,#0 : Γ, A :: Sort@s }})
+| eq_sub_eta : `({{ Γ ⊢s σ : Δ, A :: Sort@s }} ->
+                 {{ Γ ⊢s σ ≡ (σ ∘ Wk),,[σ]#0 : Δ, A :: Sort@s }})
 (* Substitution propagation *)
 | eq_sub_prop_id_left : `({{ Γ ⊢s σ : Δ }} ->
                           {{ Γ ⊢s Id ∘ σ ≡ σ : Δ }})
@@ -159,13 +160,13 @@ with eq_sub {P : PtsSig} : Ctx P -> Sub P -> Sub P -> Ctx P -> Prop :=
                            {{ Γ ⊢s σ ∘ Id ≡ σ : Δ }})
 | eq_sub_prop_assoc : `({{ Γ1 ⊢s σ1 : Γ2 }} -> {{ Γ2 ⊢s σ2 : Γ3 }} -> {{ Γ3 ⊢s σ3 : Γ4 }} ->
                         {{ Γ1 ⊢s (σ1 ∘ σ2) ∘ σ3 ≡ σ1 ∘ (σ2 ∘ σ3) : Γ4 }})
-| eq_sub_prop_ext_left : `({{ Γ ⊢s σ : Δ }} -> {{ Δ ⊢ A }} -> {{ Γ ⊢ M : [σ]A }} ->
+| eq_sub_prop_ext_left : `({{ Γ ⊢s σ : Δ }} -> {{ Δ ⊢ A : K :: L }} -> {{ Γ ⊢ M : [σ]A :: K }} ->
                            {{ Γ ⊢s (σ,,M) ∘ Wk ≡ σ : Δ }})
-| eq_sub_prop_ext_right : `({{ Γ1 ⊢s σ1 : Γ2 }} -> {{ Γ2 ⊢s σ2 : Γ3 }} -> {{ Γ3 ⊢ A : Sort@s }} -> {{ Γ2 ⊢ M : [σ2]A }} ->
-                            {{ Γ1 ⊢s σ1 ∘ (σ2,,M) ≡ (σ1 ∘ σ2),,[σ1]M : Γ3, A:s }})
+| eq_sub_prop_ext_right : `({{ Γ1 ⊢s σ1 : Γ2 }} -> {{ Γ2 ⊢s σ2 : Γ3 }} -> {{ Γ3 ⊢ A : Sort@s :: K }} -> {{ Γ2 ⊢ M : [σ2]A :: Sort@s }} ->
+                            {{ Γ1 ⊢s σ1 ∘ (σ2,,M) ≡ (σ1 ∘ σ2),,[σ1]M : Γ3, A :: Sort@s }})
 (* Congruence rules *)
-| eq_sub_cong_ext : `({{ Γ ⊢s σ1 ≡ σ2 : Δ }} -> {{ Δ ⊢ A : Sort@s }} -> {{ Γ ⊢ M1 ≡ M2 : [σ]A }} ->
-                      {{ Γ ⊢s σ1,,M1 ≡ σ2,,M2 : Δ, A:s }})
+| eq_sub_cong_ext : `({{ Γ ⊢s σ1 ≡ σ2 : Δ }} -> {{ Δ ⊢ A : Sort@s :: K }} -> {{ Γ ⊢ M1 ≡ M2 : [σ]A :: Sort@s }} ->
+                      {{ Γ ⊢s σ1,,M1 ≡ σ2,,M2 : Δ, A :: Sort@s }})
 | eq_sub_cong_comp : `({{ Γ1 ⊢s σ1 ≡ σ2 : Γ2 }} -> {{ Γ2 ⊢s τ1 ≡ τ2 : Γ3 }} ->
                        {{ Γ1 ⊢s σ1 ∘ τ1 ≡ σ2 ∘ τ2 : Γ3 }})
 (* Equivalence relation rules *)
@@ -178,4 +179,4 @@ with eq_sub {P : PtsSig} : Ctx P -> Sub P -> Sub P -> Ctx P -> Prop :=
 (* Conversion rule *)
 | eq_sub_conv : `({{ Γ ⊢s σ1 ≡ σ2 : Δ1 }} -> {{ ⊢ Δ1 ≡ Δ2 }} ->
                   {{ Γ ⊢s σ1 ≡ σ2 : Δ2 }})
-where "Γ ⊢s σ ≡ τ : Δ" := (eq_sub Γ σ τ Δ) (in custom judg) : type_scope.
+where "Γ ⊢s σ ≡ τ : Δ" := (eq_sub Γ Δ σ τ) (in custom judg) : type_scope.
