mechanization/theories/Core/Syntactic/System/Lemmas.v
@@ -1,11 +1,10 @@
-From McPTS Require Import LibTactics.
+From McPTS Require Import PtsSignature LibTactics.
 From McPTS.Core Require Import Base.
-From McPTS.Core.PTSSignature Require Import Signature.
 From McPTS.Core.Syntactic.System Require Import Definitions.
 
 (* Basic properties of contexts *)
 Lemma ctx_lookup_lt {P : PtsSig} : forall {Γ : Ctx P} {x : nat} {A : Typ P} {s : St P},
-      {{ #x : A : s ∈ Γ }} ->
+      {{ #x : A :: Sort@s ∈ Γ }} ->
       x < length Γ.
 Proof.
   induction 1; simpl; lia.
@@ -15,8 +14,8 @@ Qed.
 
 
 Lemma functional_ctx_lookup {P : PtsSig} : forall {Γ : Ctx P} {x A A' s},
-    {{ #x : A : s ∈ Γ }} ->
-    {{ #x : A' : s ∈ Γ }} ->
+    {{ #x : A :: Sort@s ∈ Γ }} ->
+    {{ #x : A' :: Sort@s ∈ Γ }} ->
     A = A'.
 Proof with mautosolve.
   intros * Hx Hx'; gen A'.
@@ -27,7 +26,7 @@ Qed.
 
 
 Lemma ctx_decomp {P : PtsSig} : forall {Γ : Ctx P} {A s},
-    {{ ⊢ Γ, A : s}} -> {{ ⊢ Γ }} /\ exists i, {{ Γ ⊢ A : Sort@i }}.
+    {{ ⊢ Γ, A :: Sort@s}} -> {{ ⊢ Γ }} /\ exists s, {{ Γ ⊢ A :: Sort@s }}.
 Proof with now eauto.
   inversion 1...
 Qed.
@@ -35,12 +34,12 @@ Qed.
 #[export]
   Hint Resolve ctx_decomp : mcpts.
 
-Corollary ctx_decomp_left {P : PtsSig} : forall {Γ : Ctx P} {A s}, {{ ⊢ Γ , A : s}} -> {{ ⊢ Γ }}.
+Corollary ctx_decomp_left {P : PtsSig} : forall {Γ : Ctx P} {A s}, {{ ⊢ Γ , A :: Sort@s}} -> {{ ⊢ Γ }}.
 Proof with easy.
   intros * ?%ctx_decomp...
 Qed.
 
-Corollary ctx_decomp_right {P : PtsSig} : forall {Γ : Ctx P} {A s}, {{ ⊢ Γ, A : s }} -> exists i, {{ Γ ⊢ A : Sort@i }}.
+Corollary ctx_decomp_right {P : PtsSig} : forall {Γ : Ctx P} {A s}, {{ ⊢ Γ, A :: Sort@s }} -> exists s, {{ Γ ⊢ A :: Sort@s }}.
 Proof with easy.
   intros * ?%ctx_decomp...
 Qed.
@@ -55,7 +54,7 @@ Hint Resolve ctx_decomp_left ctx_decomp_right : mcpts.
 
 Lemma presup_ctx_eq {P : PtsSig} : forall {Γ Δ : Ctx P}, {{ ⊢ Γ ≡ Δ }} -> {{ ⊢ Γ }} /\ {{ ⊢ Δ }}.
 Proof with mautosolve.
-  induction 1; split; econstructor; destruct_pairs; assumption.
+  induction 1; split; econstructor; destruct_pairs; mauto; econstructor; mauto.
 Qed.
 
 Corollary presup_ctx_eq_left {P : PtsSig} : forall {Γ Δ : Ctx P}, {{ ⊢ Γ ≡ Δ }} -> {{ ⊢ Γ }}.
@@ -73,7 +72,7 @@ Hint Resolve presup_ctx_eq presup_ctx_eq_left presup_ctx_eq_right : mcpts.
 
 Lemma presup_sub {P : PtsSig}: forall {Γ Δ : Ctx P} {σ}, {{ Γ ⊢s σ : Δ }} -> {{ ⊢ Γ }} /\ {{ ⊢ Δ }}.
 Proof with mautosolve.
-  induction 1; split; mauto; destruct_pairs; mauto; econstructor; assumption.
+  induction 1; split; mauto; destruct_pairs; mauto; econstructor; mauto; econstructor; mauto.
 Qed.
 
 Corollary presup_sub_left {P : PtsSig} : forall {Γ Δ : Ctx P} {σ}, {{ Γ ⊢s σ : Δ }} -> {{ ⊢ Γ }}.
@@ -91,7 +90,7 @@ Hint Resolve presup_sub presup_sub_left presup_sub_right : mcpts.
 
 (** With [presup_sub], we can prove similar for [exp]. *)
 
-Lemma presup_exp_ctx {P : PtsSig} : forall {Γ : Ctx P} {M A}, {{ Γ ⊢ M : A }} -> {{ ⊢ Γ }}.
+Lemma presup_exp_ctx {P : PtsSig} : forall {Γ : Ctx P} {M A K}, {{ Γ ⊢ M : A :: K }} -> {{ ⊢ Γ }}.
 Proof with mautosolve.
   induction 1...
 Qed.
@@ -103,7 +102,7 @@ Hint Resolve presup_exp_ctx : mcpts.
 
 Lemma presup_sub_eq_ctx {P : PtsSig} : forall {Γ Δ : Ctx P} {σ σ'}, {{ Γ ⊢s σ ≡ σ' : Δ }} -> {{ ⊢ Γ }} /\ {{ ⊢ Δ }}.
 Proof with mautosolve.
-  induction 1; split; mauto; try econstructor; mauto; destruct_pairs; mauto.
+  induction 1; split; mauto; try econstructor; mauto; destruct_pairs; mauto; econstructor; mauto.
 Qed.
 
 Corollary presup_sub_eq_ctx_left {P : PtsSig} : forall {Γ Δ : Ctx P} {σ σ'}, {{ Γ ⊢s σ ≡ σ' : Δ }} -> {{ ⊢ Γ }}.
@@ -119,7 +118,7 @@ Qed.
 #[export]
 Hint Resolve presup_sub_eq_ctx presup_sub_eq_ctx_left presup_sub_eq_ctx_right : mcpts.
 
-Lemma presup_exp_eq_ctx {P : PtsSig} : forall {Γ : Ctx P} {M M' A}, {{ Γ ⊢ M ≡ M' : A }} -> {{ ⊢ Γ }}.
+Lemma presup_exp_eq_ctx {P : PtsSig} : forall {Γ : Ctx P} {M M' A K}, {{ Γ ⊢ M ≡ M' : A :: K }} -> {{ ⊢ Γ }}.
 Proof with mautosolve 2.
   induction 1...
 Qed.
@@ -129,16 +128,15 @@ Hint Resolve presup_exp_eq_ctx : mcpts.
 
 (** *** Immediate Results of Context Presuppositions *)
 
-Lemma wf_conv {P : PtsSig} : forall (Γ : Ctx P) M A i A',
-    {{ Γ ⊢ M : A }} ->
+Lemma wf_conv {P : PtsSig} : forall (Γ : Ctx P) M A A' K L,
+    {{ Γ ⊢ M : A :: K }} ->
     (** The next argument will be removed in SystemOpt *)
-    {{ Γ ⊢ A' : Sort@i }} ->
-    {{ Γ ⊢ A ≡ A' : Sort@i }} ->
-    {{ Γ ⊢ M : A' }}.
+    {{ Γ ⊢ A' : K :: L }} ->
+    {{ Γ ⊢ A ≡ A' : K :: L }} ->
+    {{ Γ ⊢ M : A' :: K }}.
 Proof.
   intros.
-  econstructor; mauto.
-  econstructor; mauto.  
+  eapply wf_exp_conv; mauto.
 Qed.
 
 #[export]
@@ -156,16 +154,15 @@ Qed.
 #[export]
 Hint Resolve wf_sub_conv : mcpts.
 
-Lemma wf_exp_eq_conv {P : PtsSig} : forall (Γ : Ctx P) M M' A A' i,
-   {{ Γ ⊢ M ≡ M' : A }} ->
+Lemma wf_exp_eq_conv {P : PtsSig} : forall (Γ : Ctx P) M M' A A' K L,
+   {{ Γ ⊢ M ≡ M' : A :: K }} ->
    (** The next argument will be removed in SystemOpt *)
-   {{ Γ ⊢ A' : Sort@i }} ->
-   {{ Γ ⊢ A ≡ A' : Sort@i }} ->
-   {{ Γ ⊢ M ≡ M' : A' }}.
+   {{ Γ ⊢ A' : K :: L }} ->
+   {{ Γ ⊢ A ≡ A' : K :: L }} ->
+   {{ Γ ⊢ M ≡ M' : A' :: K }}.
 Proof. 
   intros.
   eapply eq_exp_conv; mauto.
-  econstructor; mauto.
 Qed.
 
 #[export]
@@ -184,22 +181,31 @@ Qed.
 Hint Resolve wf_sub_eq_conv : mcpts.
 
 
-(*  I don't understand how to port this to the PTS setting
+Lemma eq_ctx_sym {P : PtsSig} : forall {Γ Δ : Ctx P},
+    {{ ⊢ Γ ≡ Δ }} ->
+    {{ ⊢ Δ ≡ Γ }}
+.
+Proof with mautosolve.
+  intros *; induction 1; econstructor; mauto.
+Qed.
 
+    
 Add Parametric Morphism {P : PtsSig} (Γ : Ctx P) : (eq_sub Γ)
     with signature eq_ctx ==> eq ==> eq ==> iff as wf_sub_eq_morphism_iff3.
 Proof.
-  intros Δ Δ' H **; split; [| symmetry in H]; mauto.
+  intros Δ1 Δ2 H σ τ.
+  split; intros; eapply eq_sub_conv; mauto.
+  apply eq_ctx_sym; mauto.
 Qed.
-*)
 
 
 Lemma ctx_eq_refl {P : PtsSig} : forall {Γ : Ctx P},
     {{ ⊢ Γ }} ->
     {{ ⊢ Γ ≡ Γ }}.
 Proof.
-  induction 1; econstructor; mauto 4.
-  econstructor; mauto.
+  induction 1; econstructor; mauto.
+  
+  econstructor; mauto 4; econstructor; mauto; econstructor; mauto.
 Qed.
 
 #[export]
@@ -208,14 +214,20 @@ Hint Resolve ctx_eq_refl : mcpts.
 
 (** *** Lemmas for [exp] of [{{{ Type@i }}}] *)
 
-Lemma exp_sub_typ {P : PtsSig} : forall {Δ Γ : Ctx P} {A σ s},
-    {{ Δ ⊢ A : Sort@s }} ->
+
+    
+Lemma exp_sub_typ {P : PtsSig} : forall {Δ Γ : Ctx P} {A σ s K},
+    {{ Δ ⊢ A : Sort@s :: K }} ->
     {{ Γ ⊢s σ : Δ }} ->
-    {{ Γ ⊢ [σ]A : Sort@s }}.
-Proof with mautosolve 3.
-  intros.
+    {{ Γ ⊢ [σ]A : Sort@s :: K}}.
+Proof with mautosolve 3.  
+  intros.  
   econstructor; mauto 3.
-  econstructor...
+  eapply wf_exp_conv; mauto.
+  eapply wf_exp_clo; mauto.
+  econstructor; mauto.
+  
+  
   (* We are missing a rule here.
    * The problem is that the rule for sorts does not apply, so there is no other choice but to find a s' such that (s : s') ∈ Ax, but that might not be the case
    *)
@@ -227,40 +239,40 @@ Hint Resolve exp_sub_typ : mcpts.
 
 Lemma presup_ctx_lookup_typ {P : PtsSig} : forall {Γ : Ctx P} {A x s},
     {{ ⊢ Γ }} ->
-    {{ #x : A : s ∈ Γ }} ->
-    {{ Γ ⊢ A : Sort@s }}.
+    {{ #x : A :: Sort@s ∈ Γ }} ->
+    {{ Γ ⊢ A :: Sort@s }}.
 Proof with mautosolve 4.
-  intros * HΓ.  
-  induction 1; inversion_clear HΓ; eapply exp_sub_typ; mauto; econstructor; econstructor; assumption.
+  intros * HΓ.
+  induction 1; inversion_clear HΓ; eapply exp_sub_typ; mauto; econstructor; mauto; econstructor; mauto.
 Qed.
 
 #[export]
 Hint Resolve presup_ctx_lookup_typ : mcpts.
 
 
-Lemma exp_eq_sub_cong_typ1 {P : PtsSig} : forall {Δ Γ : Ctx P} {A A' σ s},
-    {{ Δ ⊢ A ≡ A' : Sort@s }} ->
+Lemma exp_eq_sub_cong_typ1 {P : PtsSig} : forall {Δ Γ : Ctx P} {A A' σ s K},
+    {{ Δ ⊢ A ≡ A' : Sort@s :: K }} ->
     {{ Γ ⊢s σ : Δ }} ->
-    {{ Γ ⊢ [σ]A ≡ [σ]A' : Sort@s }}.
+    {{ Γ ⊢ [σ]A ≡ [σ]A' : Sort@s :: K }}.
 Proof with mautosolve 3.
   intros.
   (* Same problem as before: we cannot just apply conversion because it gives [σ]Sort@s *)
 Admitted.
 
-Lemma exp_eq_sub_cong_typ2' {P : PtsSig} : forall {Δ Γ : Ctx P} {A σ τ s},
-    {{ Δ ⊢ A : Sort@s }} ->
+Lemma exp_eq_sub_cong_typ2' {P : PtsSig} : forall {Δ Γ : Ctx P} {A σ τ s K},
+    {{ Δ ⊢ A : Sort@s :: K }} ->
     {{ Γ ⊢s σ : Δ }} ->
     {{ Γ ⊢s σ ≡ τ : Δ }} ->
-    {{ Γ ⊢ [σ]A ≡ [τ]A : Sort@s }}.
+    {{ Γ ⊢ [σ]A ≡ [τ]A : Sort@s :: K }}.
 Proof with mautosolve 3.
   (* Same problem as before *)
 Admitted.
 
-Lemma exp_eq_sub_compose_typ {P : PtsSig} : forall {Ψ Δ Γ : Ctx P} {A σ τ s},
-    {{ Ψ ⊢ A : Sort@s }} ->
+Lemma exp_eq_sub_compose_typ {P : PtsSig} : forall {Ψ Δ Γ : Ctx P} {A σ τ s K},
+    {{ Ψ ⊢ A : Sort@s :: K }} ->
     {{ Δ ⊢s σ : Ψ }} ->
     {{ Γ ⊢s τ : Δ }} ->
-    {{ Γ ⊢ [σ][τ]A ≡ [σ∘τ]A : Sort@s }}.
+    {{ Γ ⊢ [σ][τ]A ≡ [σ∘τ]A : Sort@s :: K }}.
 Proof with mautosolve 3.
   (* Same problem *)
 Admitted.
@@ -268,22 +280,40 @@ Admitted.
 #[export]
 Hint Resolve exp_eq_sub_cong_typ1 exp_eq_sub_cong_typ2' exp_eq_sub_compose_typ : mcpts.
 
-Lemma exp_eq_sub_compose_weaken_extend_typ {P : PtsSig} : forall {Γ : Ctx P} {σ Δ s1 A s2 B M},
+Lemma exp_eq_sub_compose_weaken_extend_typ {P : PtsSig} : forall {Γ : Ctx P} {σ Δ s1 A s2 B M K1 K2},
     {{ Γ ⊢s σ : Δ }} ->
-    {{ Δ ⊢ A : Sort@s1 }} ->
-    {{ Δ ⊢ B : Sort@s2 }} ->
-    {{ Γ ⊢ M : [σ]B }} ->
-    {{ Γ ⊢ [Wk][σ,,M]A ≡ [σ]A : Sort@s1 }}.
+    {{ Δ ⊢ A : Sort@s1 :: K1 }} ->
+    {{ Δ ⊢ B : Sort@s2 :: K2 }} ->
+    {{ Γ ⊢ M : [σ]B :: Sort@s2}} ->
+    {{ Γ ⊢ [Wk][σ,,M]A ≡ [σ]A : Sort@s1 :: K1 }}.
 Proof with mautosolve 3.
-  intros.
-  assert {{ Δ, B : s2 ⊢s Wk : Δ }}.
-  {
-    econstructor; mauto.
-    econstructor; mauto.
-  }
   (* Same problem *)
 Admitted.
 
 #[export]
 Hint Resolve exp_eq_sub_compose_weaken_extend_typ : mcpts.
 
+
+Lemma exp_eq_sub_compose_weaken_id_extend_typ {P : PtsSig} : forall {Γ : Ctx P} {s1 A s2 B M K1 K2},
+    {{ Γ ⊢ A : Sort@s1 :: K1 }} ->
+    {{ Γ ⊢ B : Sort@s2 :: K2 }} ->
+    {{ Γ ⊢ M : B :: Sort@s2 }} ->
+    {{ Γ ⊢ [Wk][Id,,M]A ≡ A : Sort@s1 :: K1 }}.
+Proof with mautosolve 4.
+  intros.  
+  assert {{ Γ ⊢ [Id]B : Sort@s2 :: K2 }}.
+  {
+    eapply wf_exp_conv.
+    eapply wf_exp_clo; mauto.
+    econstructor.
+    mauto.
+    eapply wf_typ_exp.
+  }
+  by mauto 4.
+  assert {{ Γ ⊢ B ⊆ B[Id] }} by mauto 4.
+  assert {{ Γ ⊢ M : B[Id] }} by mauto 2.
+  transitivity {{{ A[Id] }}}...
+Qed.
+
+#[export]
+Hint Resolve exp_eq_sub_compose_weaken_id_extend_typ : mcpts.
